
| **Category**         | **Law (Name)**   | **Formula**                                                                                      |
| -------------------- | ---------------- | ------------------------------------------------------------------------------------------------ |
| **Basic Identities** | Identity Law     | $p \land T \equiv p$<br>$p \lor F \equiv p$                                                      |
|                      | Domination Law   | $p \lor T \equiv T$<br>$p \land F \equiv F$                                                      |
|                      | Idempotent Law   | $p \lor p \equiv p$<br>$p \land p \equiv p$                                                      |
|                      | Double Negation  | $¬(¬p) \equiv p$                                                                                 |
| **Commutative**      | OR/AND swap      | $p \lor q \equiv q \lor p$<br>$p \land q \equiv q \land p$                                       |
| **Associative**      | OR/AND regroup   | $(p \lor q) \lor r \equiv p \lor (q \lor r)$<br>$(p \land q) \land r \equiv p \land (q \land r)$ |
| **Distributive**     | AND over OR      | $p \land (q \lor r) \equiv (p \land q) \lor (p \land r)$                                         |
|                      | OR over AND      | $p \lor (q \land r) \equiv (p \lor q) \land (p \lor r)$                                          |
| **Absorption**       |                  | $p \lor (p \land q) \equiv p$<br>$p \land (p \lor q) \equiv p$                                   |
| **Negation**         | Contradiction    | $p \land ¬p \equiv F$                                                                            |
|                      | Excluded Middle  | $p \lor ¬p \equiv T$                                                                             |
| **De Morgan’s**      |                  | $¬(p \land q) \equiv (¬p \lor ¬q)$<br>$¬(p \lor q) \equiv (¬p \land ¬q)$                         |
| **Implication**      | Definition of →  | $p \to q \equiv ¬p \lor q$                                                                       |
|                      | Contrapositive   | $p \to q \equiv ¬q \to ¬p$                                                                       |
|                      | Converse         | $q \to p$ (not equivalent to $p \to q$)                                                          |
| **Biconditional**    | Definition of ↔  | $p \leftrightarrow q \equiv (p \to q) \land (q \to p)$                                           |
|                      | Alternative Form | $p \leftrightarrow q \equiv (p \land q) \lor (¬p \land ¬q)$                                      |
